\textbf{\hypertarget{P3}{[\,Suggested Time: 15 mins \textbar \, Total Marks: 10 \textbar \, Intermediate\,]}}\\
    The first three terms of the expansion \(\displaystyle (2-x)\left(2+\frac{x^{2}}{4}\right)^{n}\left(4+2x+x^{2}\right)\) is \(a+ax^{2}-bx^{3}\), \\
    where \(n\in \mathbb{Z}^{+}, n\geq 2\). Find the values of \(a, b, n\).
    \qnmark{10}

%%%%%%%%%%%%%%%%%%
%%%%%Solution%%%%%
%%%%%%%%%%%%%%%%%%

%\begin{comment}

%%%%%Rewriting the Equation%%%%%
\begin{gather*}
    \displaystyle (2-x)\left(4+2x+x^{2}\right) = \left(8-x^{3}\right) \wrkonemark \\
    \displaystyle \therefore (2-x)\left(2+\frac{x^{2}}{4}\right)^{n}\left(4+2x+x^{2}\right) = \left(8-x^{3}\right)\left(2+\frac{x^{2}}{4}\right)^{n} \wrkonemark \\
\end{gather*}

%%%%%Finding the first 2 terms of the n power binomial%%%%%
Finding the first 2 terms of \(\displaystyle \left(2+\frac{x^{2}}{4}\right)^{n}\),
\begin{align*}
    \displaystyle \left(2+\frac{x^{2}}{4}\right)^{n} &= \sum_{r=0}^{n} \binom{n}{r}(2)^{n-r}\left(\frac{x^{2}}{4}\right)^{r} \wrkonemark \\
    \displaystyle                                    &= \sum_{r=0}^{n} \binom{n}{r}(2)^{n-3r}(x)^{2r} \\
    \displaystyle                                    &= 2^{n}+2^{n-3}(n)x^{2}+\cdots \wrkonemark \\
\end{align*}

%%%%%Finding a,b,n%%%%%
\begin{multicols}{2}
    Comparing coeff. of const. term
    \begin{gather*}
        \displaystyle 8\left(2^{n}\right) = a \tag*{(1)} \\ \wrkonemark
    \end{gather*}

    Comparing coeff. of \(x^{2}\)
    \begin{gather*}
        \displaystyle 8n\left(2^{n-3}\right) = a \tag*{(2)} \\ \wrkonemark
    \end{gather*}
\end{multicols}

\begin{multicols}{2}
    Sub (1) into (2),
    \begin{align*}
        \displaystyle             8\left(2^{n}\right) &= 8n\left(2^{n-3}\right) \wrkonemark \\
        \displaystyle        2^{n}-\frac{n}{8}(2^{n}) &= 0 \\
        \displaystyle 2^{n}\left(1-\frac{n}{8}\right) &= 0
    \end{align*}
    \begin{gather*}
        \displaystyle \therefore 2^{n} = 0 \quad or \quad \frac{n}{8} = 1 \\
        \displaystyle \hspace*{13pt} (Rej.) \\
        \displaystyle \text{Hence,} \; n = 8 \ansonemark
    \end{gather*}

    Sub \(n=8\) into (1),
    \begin{align*}
        \displaystyle \therefore a &= 8\left(2^{8}\right) \\
        \displaystyle              &= 2048 \ansonemark \\
    \end{align*}

    Comparing coeff. of \(x^{3}\)
    \begin{align*}
        \displaystyle           -b &= -2^{8} \\
        \displaystyle \therefore b &= 256 \ansonemark \\
    \end{align*}
\end{multicols}


Therefore, \(n=8, a=2048, b=256\)

%\end{comment}

\newpage \ \newpage %Do not Comment